Spacetalk/Vector.lean
@@ -1,24 +1,26 @@
 import Mathlib.Tactic.Linarith.Frontend
 import Mathlib.Data.Vector.Basic
 
+open Mathlib
+open Vector
+
 theorem Vector.get_append_left {xs : Vector α n} {ys : Vector α m} {i : Fin n}
-  : (xs.append ys).get ⟨i, by apply Nat.lt_add_right; exact i.isLt⟩ = xs.get i := by
-  apply List.get_append_left
+  : (xs.append ys).get ⟨i, Nat.lt_add_right _ i.isLt⟩ = xs.get i := by
+  apply List.getElem_append_left
+
+theorem Vector.toList_get {v : Vector α n} {i : Fin n} : v.get i = v.toList.get ⟨i, v.toList_length.symm ▸ i.isLt⟩ := by
+  cases v; simp [Vector.get]
 
 theorem Vector.get_append_right {xs : Vector α n} {ys : Vector α m} {i : Fin m}
-  : (xs.append ys).get ⟨i + n, by have := i.isLt; linarith⟩ = ys.get i := by
-  simp_rw [Vector.get_eq_get]
-  have := Vector.toList_append xs ys
-  rw [List.get_of_eq this]
-  simp [Fin.cast]
-  have := List.get_append_right xs.toList ys.toList (i := i + n)
-  have h_i_lt_append : ↑i + n < (xs.toList ++ ys.toList).length := by have := i.isLt; simp; linarith
-  have h_i_sub_xs_lt_ys : ↑i + n - xs.toList.length < ys.toList.length := by simp
-  have : List.get (xs.toList ++ ys.toList) ⟨↑i + n, h_i_lt_append⟩ = List.get ys.toList ⟨i + n - xs.toList.length, h_i_sub_xs_lt_ys⟩ := this (by rw [Vector.toList_length xs]; linarith)
-  have h_eq : (⟨↑i + n - xs.toList.length, h_i_sub_xs_lt_ys⟩ : Fin ys.toList.length) = ⟨↑i, Fin.cast.proof_1 (toList_length ys).symm i⟩ := by simp
-  rw [←h_eq]
-  exact this
-
--- @[simp]
--- theorem Vector.length_append (as : Vector α n) (bs : Vector α m) : (as.append bs).length = n + m := by
---   simp
+  : (xs.append ys).get ⟨i + n, by have := i.isLt; linarith⟩ = ys.get i :=
+  match xs, ys with
+  | ⟨xsl, xeq⟩, ⟨ysl, yeq⟩ => by
+    simp [Vector.get]
+    have := List.getElem_append_right (i := i + n) xsl ysl
+    rw [xeq] at this
+    simp at this
+    apply this
+    have ilt := i.isLt
+    linarith
+    rw [yeq]
+    exact i.isLt
